Add context as a parameter to eval_once, update on evaluation.

DlangLean/Stlc.lean
@@ -44,12 +44,12 @@ def substitute {α : Type} {σ : Type} {f_ty : α → Option σ} (with_expr : @E
 -- The size of the type tree will strictly decrease
 -- it literally cannot get bigger
 -- This is how we do structural recursion
-def eval_once {α : Type} {σ : Type} {f_ty : α → Option σ} : @Expr α σ f_ty → @Expr α σ f_ty
-  | app (abstraction _ body) rhs =>
-    substitute rhs body
+def eval_once {α : Type} {σ : Type} {f_ty : α → Option σ} (ctx : Context $ @Ty σ) : @Expr α σ f_ty → (Context $ @Ty σ) × @Expr α σ f_ty
+  | app (abstraction bind_ty body) rhs =>
+    ⟨bind_ty::ctx, substitute rhs body⟩
   | app lhs rhs =>
-    app (eval_once lhs) rhs
-  | x => x
+    ⟨ctx, app (eval_once ctx lhs).2 rhs⟩
+  | x => ⟨ctx, x⟩
 
 def valid_typing_judgements {α : Type} {σ : Type} {f_ty : α → Option σ} (ctx : Context $ @Ty σ) : @Expr α σ f_ty → Set (@Ty σ)
   | var n =>
@@ -59,25 +59,25 @@ def valid_typing_judgements {α : Type} {σ : Type} {f_ty : α → Option σ} (c
       | base t => f_ty v = some t
       | _ => false }
   | app lhs rhs =>
-    { t | ∃ ty_lhs ty_rhs, ty_rhs ∈ valid_typing_judgements ctx rhs → ty_lhs ∈ valid_typing_judgements ctx lhs → ty_lhs = arrow ty_rhs t }
+    { t | ∃ ty_lhs ty_rhs, ty_rhs ∈ valid_typing_judgements ctx rhs ∧ ty_lhs ∈ valid_typing_judgements ctx lhs ∧ ty_lhs = arrow ty_rhs t }
   | abstraction bind_ty body =>
-    { t | ∃ body_ty, (body_ty : @Ty σ) ∈ valid_typing_judgements ctx body → t = arrow bind_ty body_ty }
+    { t | ∃ body_ty, (body_ty : @Ty σ) ∈ valid_typing_judgements ctx body ∧ t = arrow bind_ty body_ty }
 
-inductive beta_normal {α : Type} {σ : Type} {f_ty : α → Option σ} (ctx : Context $ @Ty σ) : Expr → Prop
-  | trivial e   : @eval_once α σ f_ty e = e     → beta_normal ctx e
-  | hard e      : beta_normal ctx (eval_once e) → beta_normal ctx e
+inductive beta_normal {α : Type} {σ : Type} {f_ty : α → Option σ} : Context (@Ty σ) → Expr → Prop
+  | trivial ctx e   : @eval_once α σ f_ty ctx e = ⟨ctx, e⟩                → beta_normal ctx e
+  | hard ctx e      : beta_normal (eval_once ctx e).1 (eval_once ctx e).2 → beta_normal ctx e
 
-inductive beta_eq {α : Type} {σ : Type} {f_ty : α → Option σ} (ctx : Context $ @Ty σ) : @Expr α σ f_ty → @Expr α σ f_ty → Prop
-  | trivial e₁ e₂    : e₁ = e₂  → beta_eq ctx e₁ e₂
-  | right   e₁ e₂    : e₁ ≠ e₂  → beta_eq ctx e₁ (eval_once e₂) → beta_eq ctx e₁ e₂
-  | left    e₁ e₂    : e₁ ≠ e₂  → beta_eq ctx (eval_once e₁) e₂ → beta_eq ctx e₁ e₂
+inductive beta_eq {α : Type} {σ : Type} {f_ty : α → Option σ} : Context (@Ty σ) → @Expr α σ f_ty → @Expr α σ f_ty → Prop
+  | trivial (_ : Context (@Ty σ))   e₁ e₂    : e₁ = e₂                                      → beta_eq ctx e₁ e₂
+  | right   ctx e₁ e₂    : e₁ ≠ e₂  → beta_eq (eval_once ctx e₂).1 e₁ (eval_once ctx e₂).2 → beta_eq ctx e₁ e₂
+  | left    ctx e₁ e₂    : e₁ ≠ e₂  → beta_eq (eval_once ctx e₁).1 (eval_once ctx e₁).2 e₂ → beta_eq ctx e₁ e₂
 
-inductive is_strongly_normalizing {α : Type} {σ : Type} {f_ty : α → Option σ} (ctx : Context $ @Ty σ) : @Expr α σ f_ty → Prop
-  | trivial (e : Expr) : eval_once e = e → is_strongly_normalizing ctx e
-  | hard    (e : Expr) : is_strongly_normalizing ctx (eval_once e) → is_strongly_normalizing ctx e
+inductive is_strongly_normalizing {α : Type} {σ : Type} {f_ty : α → Option σ} : Context (@Ty σ) → @Expr α σ f_ty → Prop
+  | trivial (ctx : Context Ty) (e : Expr) : eval_once ctx e = ⟨ctx, e⟩                                      → is_strongly_normalizing ctx e
+  | hard    (ctx : Context Ty) (e : Expr) : is_strongly_normalizing (eval_once ctx e).1 (eval_once ctx e).2 → is_strongly_normalizing ctx e
 
 
-lemma eval_once_noop_not_app {α : Type} {σ : Type} {f_ty : α → Option σ} (e : @Expr α σ f_ty) (h_not_app : match e with | app _ _ => false | _ => true) : eval_once e = e := by
+lemma eval_once_noop_not_app {α : Type} {σ : Type} {f_ty : α → Option σ} (ctx : Context Ty) (e : @Expr α σ f_ty) (h_not_app : match e with | app _ _ => false | _ => true) : eval_once ctx e = ⟨ctx, e⟩ := by
   match e with
     | var _ =>
       unfold eval_once
@@ -91,7 +91,7 @@ lemma eval_once_noop_not_app {α : Type} {σ : Type} {f_ty : α → Option σ} (
       unfold eval_once
       rfl
 
-lemma eval_once_noop_judgement_holds {α : Type} {σ : Type} {f_ty : α → Option σ} (ctx : Context $ @Ty σ) (e : @Expr α σ f_ty) (h_not_app : match e with | app _ _ => false | _ => true) : ∀ t, t ∈ @valid_typing_judgements α σ f_ty ctx e → t ∈ valid_typing_judgements ctx (eval_once e) := by
+lemma eval_once_noop_judgement_holds {α : Type} {σ : Type} {f_ty : α → Option σ} (ctx : Context Ty) (e : @Expr α σ f_ty) (h_not_app : match e with | app _ _ => false | _ => true) : ∀ t, t ∈ @valid_typing_judgements α σ f_ty ctx e → t ∈ valid_typing_judgements (eval_once ctx e).1 (eval_once ctx e).2 := by
   match h : e with
     | var _ =>
       simp [eval_once_noop_not_app]
@@ -102,4 +102,48 @@ lemma eval_once_noop_judgement_holds {α : Type} {σ : Type} {f_ty : α → Opti
     | const _ =>
       simp [eval_once_noop_not_app]
 
-lemma eval_once_judgement_holds {α : Type} {σ : Type} {f_ty : α → Option σ} (ctx : Context $ @Ty σ) : ∀ e t, t ∈ @valid_typing_judgements α σ f_ty ctx e → t ∈ valid_typing_judgements ctx (eval_once e) := sorry
+lemma eval_once_judgement_holds {α : Type} {σ : Type} {f_ty : α → Option σ} (ctx : Context $ @Ty σ) : ∀ e t, t ∈ @valid_typing_judgements α σ f_ty ctx e → t ∈ valid_typing_judgements ctx (eval_once e)
+  | e, t, h_t =>
+    match h : e with
+      | var n =>
+        eval_once_noop_judgement_holds ctx (var n) (by simp_all) t h_t
+      | app lhs rhs => by
+        -- Hard case:
+        -- we know that given t is a valid typing judgement,
+        -- the type of the lhs is arrow rhs -> t
+        -- and the type of the entire expression is the type of body
+        unfold valid_typing_judgements at h_t
+        simp at h_t
+        have ⟨ty_lhs, ty_rhs, ⟨h_ty_rhs, h_t_lhs, h_t'⟩⟩ := h_t
+        unfold eval_once
+        match lhs with
+          | abstraction bind_ty body =>
+            unfold substitute
+            unfold valid_typing_judgements
+            simp
+            unfold valid_typing_judgements at h_t_lhs
+            simp at h_t_lhs
+            have ⟨body_ty, h_body_ty⟩ := h_t_lhs
+            simp_all
+            have ⟨h_t_rhs', h_t_body'⟩ := h_t'
+            split
+            
+            sorry
+          | var n =>
+            simp
+            unfold eval_once
+            unfold valid_typing_judgements
+            simp
+            exact h_t
+          | const _ =>
+            simp
+            unfold eval_once
+            unfold valid_typing_judgements
+            simp
+            exact h_t
+          | app _ _ =>
+            sorry
+      | abstraction bind_ty body=>
+        eval_once_noop_judgement_holds ctx (abstraction bind_ty body) (by simp_all) t h_t
+      | const e =>
+        eval_once_noop_judgement_holds ctx (const e) (by simp_all) t h_t
